Minor

src/circuits/dependent_test.lean
@@ -82,6 +82,58 @@ lemma _root_.tencodable.encode_sigma (x : α) (y : β x) : encode (⟨x, y⟩ : 
 
 end complexity_class
 
+/-- A function which is encoded as a table -/
+structure complexity_class.table_fun (α β : Type*) :=
+(to_fun : α → β)
+
+namespace complexity_class.table_fun
+open_locale complexity_class
+variables {α β γ : Type*}
+
+localized "infixr ` [→] `:25 := complexity_class.table_fun" in complexity_class
+
+instance : has_coe_to_fun (α [→] β) (λ _, α → β) := ⟨table_fun.to_fun⟩
+
+@[ext]
+protected lemma ext : ∀ (f g : α [→] β), ⇑f = (by exact ⇑g) → f = g
+| ⟨f⟩ ⟨g⟩ rfl := rfl
+
+@[simp] lemma to_fun_eq_coe (f : α [→] β) : f.to_fun = ⇑f := rfl
+
+@[simps]
+def equiv_fun : (α [→] β) ≃ (α → β) := ⟨λ f, ⇑f, λ f, ⟨f⟩, λ f, by ext; refl, λ f, rfl⟩
+
+@[simps]
+def sum (f : α [→] γ) (g : β [→] γ) : α ⊕ β [→] γ := ⟨sum.elim ⇑f ⇑g⟩
+
+@[simps]
+def map (f : α [→] β) (g : β → γ) : α [→] γ := ⟨λ x, g (f x)⟩
+
+@[simps]
+def comp (f : α [→] β) (g : γ [→] α) : γ [→] β := ⟨λ x, f (g x)⟩
+
+def finmap_equiv_fun [fintype α] [decidable_eq α] :
+  {x : @finmap α (λ _, β) // ∀ k : α, k ∈ x} ≃ (α → β) :=
+{ to_fun := λ f x, @option.get _ ((↑f : finmap _).lookup x) (finmap.lookup_is_some.mpr $ f.prop x),
+  inv_fun := λ f, ⟨finmap.of_fun f, λ k, finmap.mem_iff.mpr ⟨_, finmap.of_fun_lookup k⟩⟩,
+  left_inv := λ f, by { ext : 1, apply finmap.ext_lookup, simp, },
+  right_inv := λ f, by { ext, simp, } } 
+
+variables [tencodable α] [fintype α] [decidable_eq α] [tencodable β] [tencodable γ]
+
+instance : tencodable (α [→] β) :=
+tencodable.of_equiv _ (equiv_fun.trans finmap_equiv_fun.symm)
+
+lemma encode_table_fun (f : α [→] β) : encode f = encode (finmap_equiv_fun.symm ⇑f) :=
+rfl
+
+lemma table_fun_mk_of {γ : Type} {ψ₁ ψ₂ : γ → Type} [tencodable γ] [∀ x, tencodable (ψ₁ x)] 
+  [∀ x, fintype (ψ₁ x)] [∀ x, decidable_eq (ψ₁ x)] [∀ x, tencodable (ψ₂ x)] {f : ∀ x, (ψ₁ x → ψ₂ x)}
+  (hψ : polytime.mem_types ψ₁) (hf : f ∈ₜ PTIME) : (λ x, table_fun.mk (f x) : ∀ x, ψ₁ x [→] ψ₂ x) ∈ₐ PTIME := 
+sorry
+
+end complexity_class.table_fun
+
 namespace polytime
 open_locale complexity_class
 open_locale tree
@@ -91,7 +143,7 @@ variables {α : Type} {β : α → Type} {β₁ : α → Type} {β₂ : α → T
   [tencodable α] [∀ x, tencodable (β x)] [∀ x, tencodable (β₁ x)] [∀ x, tencodable (β₂ x)]
   [tencodable γ] [tencodable δ] {C : complexity_class}
 
-lemma list_map_dep {l : ∀ x, list (β₁ x)} {f : ∀ x, β₁ x → β₂ x} (hl : l ∈ₐ PTIME)
+@[complexity] lemma list_map_dep {l : ∀ x, list (β₁ x)} {f : ∀ x, β₁ x → β₂ x} (hl : l ∈ₐ PTIME)
   (hf : f ∈ₜ PTIME) : (λ x : α, (l x).map (f x) : ∀ x, list (β₂ x)) ∈ₐ PTIME :=
 begin
   rcases hf with ⟨f', pf, hf⟩,
@@ -100,6 +152,8 @@ begin
   simp at hf, dsimp [tencodable.encode_sigma] at hf, simp [function.comp, hf],
 end
 
-
+@[complexity] lemma list_append_dep {l₁ l₂ : ∀ x, list (β x)} (hl₁ : l₁ ∈ₐ PTIME) (hl₂ : l₂ ∈ₐ PTIME) :
+  (λ x, (l₁ x) ++ (l₂ x)) ∈ₐ PTIME :=
+by { rw [mem_iff_comp_list_encode_dep] at *, simp only [list.map_append], complexity, }
 
 end polytime
